<p>There are two integer arrays <strong>A</strong> and <strong>B</strong>. The length of array <strong>A</strong> is <strong>n </strong>and length of array <strong>B</strong>&nbsp;is <strong>k</strong>. Array <strong>A&nbsp;</strong>= <strong>[</strong> <strong>a<sub>1&nbsp;</sub>, a<sub>2&nbsp;</sub>,</strong> <strong>...</strong> <strong>,</strong>&nbsp;<strong>a<sub>i</sub>&nbsp;... , a<span style="font-size: 8.33333px;"><sub>n</sub></span>&nbsp;] </strong>and <strong>B</strong><strong>&nbsp;</strong>=&nbsp;<strong>[</strong>&nbsp;<strong>b</strong><strong><sub>1&nbsp;</sub>, b<sub>2&nbsp;</sub>,</strong>&nbsp;<strong>...</strong>&nbsp;<strong>,</strong>&nbsp;<strong>b<span style="font-size: 8.33333px;">j</span></strong><strong>&nbsp;... , b<sub>k</sub>&nbsp;]&nbsp; </strong>where <strong>1 &lt;=</strong> <strong>a<sub>i</sub></strong>&nbsp;<strong>&lt;= k</strong> and <strong>1 &lt;=</strong> <strong>b<span style="font-size: 8.33333px;">j</span></strong>&nbsp;<strong>&lt;= n</strong> and <strong>1 &lt;= i &lt;= n</strong> and <strong>1 &lt;= j &lt;= k</strong> and <strong>1 &lt;= k &lt;= n &lt;= 10<sup>7</sup></strong>. If there exists a subarray of <strong>A</strong> which has the same sum as some subarray of <strong>B </strong><strong>then</strong><strong> <strong>B </strong><strong>and</strong><strong> </strong><strong>A </strong>are said to be&nbsp;</strong><strong><strong><strong>twisted</strong><strong> arrays</strong></strong><strong>.</strong></strong></p>
<p>More mathematically, if there exists <strong>p</strong>, <strong>q</strong>, <strong>r</strong> and <strong>s</strong> such that <strong>sum</strong>(<strong>A</strong>, <strong>p</strong>, <strong>q</strong>) = <strong>sum</strong>(<strong>B</strong>, <strong>r</strong>, <strong>s</strong>), where <strong>1 &lt;= p &lt;= q &lt;= n </strong>and <strong>1 &lt;= r &lt;= s &lt;= k </strong>and <strong>sum(A, p, q)</strong> = <strong>a<sub>p </sub>&nbsp;+ a<sub>p+1 </sub></strong>&nbsp;+ <strong>a</strong><sub><strong>p+2</strong>&nbsp;</sub><strong>...</strong>&nbsp;+&nbsp;<strong>a<sub>q-1</sub></strong><strong>&nbsp;+ a<sub>q</sub></strong>&nbsp; and <strong>sum(B, r, s)</strong> = <strong>b</strong><strong><sub>r&nbsp;</sub>&nbsp;+ b<sub>r+1&nbsp;</sub></strong>&nbsp;+ <strong>b</strong><sub><strong>r+2</strong>&nbsp;</sub><strong>...</strong>&nbsp;+&nbsp;<strong>b</strong><strong><sub>s-1</sub></strong><strong><strong>&nbsp;+ b</strong><sub>s</sub><sub><strong>&nbsp;</strong>then the two arrays<strong> A and B</strong> are said to be<strong> twisted arrays.</strong></sub></strong></p>
<h3>Input</h3>
<p>Input contains <strong>n + k + 1</strong> lines. The first line has values for <strong>n</strong> and <strong>k </strong>separated by space.</p>
<p>Then next <strong>n</strong> lines specify the elements of array <strong>A</strong>. The next <strong>k</strong> lines specify the elements of array <strong>B.</strong></p>
<h3>Output</h3>
<p>One line containing <strong>Yes </strong>if the arrays are <strong>twisted</strong>&nbsp;or&nbsp;<strong>No </strong>otherwise (Note:&nbsp;<strong>Yes</strong> and <strong>No</strong> are case sensitive)</p>
<h3>Example</h3>
<pre><strong>Input:</strong>
<p>4 3<br>1<br>2<br>3<br>1<br>2<br>1<br>1</p></pre>
<pre><strong>Output:<br></strong>Yes</pre>
<p><strong>&nbsp;</strong></p>
<pre><strong>Explanation:</strong></pre>
<pre>Here A = [1, 2, 3, 1] and B = [2, 1, 1]. Clearly a<sub>1</sub> + a<sub>2</sub> = b<sub>1</sub> + b<sub>2 </sub>. And so A and B are twisted</pre>